theories/par.v
@@ -34,34 +34,7 @@ Inductive TyPar : Ty -> Ty -> Type :=
   (* -------------------------------------- *)
   TyPar (TyForall k a0) (TyForall k a1).
 
-
-Reserved Infix "⇒" (at level 70, no associativity).
-Inductive Par : Tm -> Tm -> Prop :=
-| P_Var i :
-  VarTm i ⇒ VarTm i
-| P_Abs a0 a1 :
-  a0 ⇒ a1 ->
-  (* ------------------- *)
-  TmAbs a0 ⇒ TmAbs a1
-| P_App a0 a1 b0 b1 :
-  a0 ⇒ a1 ->
-  b0 ⇒ b1 ->
-  TmApp a0 b0 ⇒ TmApp a1 b1
-| P_AppAbs a0 a1 b0 b1 :
-  a0 ⇒ a1 ->
-  b0 ⇒ b1 ->
-  (* ---------------------------------- *)
-  TmApp (TmAbs a0) b0 ⇒ subst_Tm (b1…) a1
-(* | P_Forall a0 a1 : *)
-(*   a0 ⇒ a1 -> *)
-(*   (* ------------------------------- *) *)
-(*   TmForall a0 ⇒ TmForall a1 *)
-
-where "a ⇒ b" := (Par a b).
-
-#[export]Hint Constructors Par TyPar : par.
-
-Infix "⇒*" := (rtc Par) (at level 70, no associativity).
+#[export]Hint Constructors TyPar : par.
 
 Inductive RTC  : Ty -> Ty -> Type :=
 | RTC_Refl A :
@@ -74,84 +47,11 @@ Inductive RTC  : Ty -> Ty -> Type :=
 Definition ICoherent A0 A1 : Type :=
   { B : Ty &  prod (RTC A0 B) (RTC A1 B)}.
 
-Lemma par_refl a : a ⇒ a.
-Proof. elim : a; eauto with par. Qed.
-
-Ltac2 binder_map (f : constr -> constr) (b : binder) : binder :=
-  Binder.make (Binder.name b) (f (Binder.type b)).
-
-Local Ltac2 map_invert (f : constr -> constr) (iv : case_invert) : case_invert :=
-  match iv with
-  | NoInvert => NoInvert
-  | CaseInvert indices => CaseInvert (Array.map f indices)
-  end.
-
-Ltac2 map (f : constr -> constr) (c : constr) : constr :=
-  match Unsafe.kind c with
-  | Rel _ | Meta _ | Var _ | Sort _ | Constant _ _ | Ind _ _
-  | Constructor _ _ | Uint63 _ | Float _  => c
-  | Cast c k t =>
-      let c := f c
-      with t := f t in
-      make (Cast c k t)
-  | Prod b c =>
-      let b := binder_map f b
-      with c := f c in
-      make (Prod b c)
-  | Lambda b c =>
-      let b := binder_map f b
-      with c := f c in
-      make (Lambda b c)
-  | LetIn b t c =>
-      let b := binder_map f b
-      with t := f t
-      with c := f c in
-      make (LetIn b t c)
-  | App c l =>
-      let c := f c
-      with l := Array.map f l in
-      make (App c l)
-  | Evar e l =>
-      let l := Array.map f l in
-      make (Evar e l)
-  | Case info x iv y bl =>
-      let x := match x with (x,x') => (f x, x') end
-      with iv := map_invert f iv
-      with y := f y
-      with bl := Array.map f bl in
-      make (Case info x iv y bl)
-  | Proj p r c =>
-      let c := f c in
-      make (Proj p r c)
-  | Fix structs which tl bl =>
-      let tl := Array.map (binder_map f) tl
-      with bl := Array.map f bl in
-      make (Fix structs which tl bl)
-  | CoFix which tl bl =>
-      let tl := Array.map (binder_map f) tl
-      with bl := Array.map f bl in
-      make (CoFix which tl bl)
-  | Array u t def ty =>
-      let ty := f ty
-      with t := Array.map f t
-      with def := f def in
-      make (Array u t def ty)
-  end.
-
-Ltac2 par_cong_rel c r :=
-  let rec go c :=
-    lazy_match! c with
-    | Par => r
-    | _ => map go c
-    end in go (type c).
-
 Ltac revert_all_terms :=
   repeat (progress
             (match goal with
                [_x : Tm |- _] => (revert _x)
              end)).
-
-Ltac2 Notation "gen_cong" x(constr) r(constr) := Control.refine (fun _ => par_cong_rel x r).
 
 Ltac solve_s_rec :=
   move => *; eapply rtc_l; eauto;
@@ -163,146 +63,6 @@ Ltac solve_pars_cong :=
             revert_all_terms;
             induction x; last by solve_s_rec);
   auto using rtc_refl.
-
-Lemma PS_App : ltac2:(gen_cong P_App (rtc Par)).
-Proof. solve_pars_cong. Qed.
-
-Lemma P_AppAbs' a0 a1 b0 b1 u :
-  u = subst_Tm (b1…) a1 ->
-  a0 ⇒ a1 ->
-  b0 ⇒ b1 ->
-  (* -------------------- *)
-  TmApp (TmAbs a0) b0 ⇒ u.
-Proof. move =>> ->. apply P_AppAbs. Qed.
-
-Lemma par_renaming a b ξ :
-  a ⇒ b ->
-  ren_Tm ξ a ⇒ ren_Tm ξ b.
-Proof.
-  move => h. move : ξ. elim : a b/h => //=; eauto with par.
-  (* Abs *)
-  - move => *. apply : P_AppAbs'; eauto. by asimpl.
-Qed.
-
-Lemma par_ρ_ext a b ρ0 ρ1 :
-  a ⇒ b ->
-  (forall i, ρ0 i ⇒ ρ1 i) ->
-  (forall i, (a .: ρ0) i ⇒ (b .: ρ1) i).
-Proof. qauto l:on inv:nat. Qed.
-
-Lemma par_ρ_id ρ :
-  forall (i : nat), ρ i ⇒ ρ i.
-Proof. eauto using par_refl. Qed.
-
-Lemma par_ρ_up ρ0 ρ1 :
-  (forall i, ρ0 i ⇒ ρ1 i) ->
-  (forall i, (up_Tm_Tm ρ0) i ⇒ (up_Tm_Tm ρ1) i).
-Proof. hauto l:on use:par_renaming, par_ρ_ext, P_Var unfold:up_Tm_Tm. Qed.
-
-Lemma par_morphing a b ρ0 ρ1 :
-  (forall i, ρ0 i ⇒ ρ1 i) ->
-  a ⇒ b ->
-  subst_Tm ρ0 a ⇒ subst_Tm ρ1 b.
-Proof.
-  move => + h. move : ρ0 ρ1.
-  elim : a b /h=>//=; eauto using par_ρ_up with par.
-  (* App *)
-  - move => *.
-    apply : P_AppAbs'; eauto using par_ρ_up. by asimpl.
-Qed.
-
-Lemma pars_morphing a b ρ0 ρ1 :
-  (forall i, ρ0 i ⇒ ρ1 i) ->
-  a ⇒* b ->
-  subst_Tm ρ0 a ⇒* subst_Tm ρ1 b.
-Proof.
-  move => h.
-  move => h0.
-  elim : a b /h0=>//=;
-    eauto using par_morphing, par_refl, rtc_once, rtc_l.
-Qed.
-
-Function tstar a :=
-  match a with
-  | VarTm _ => a
-  | TmAbs a => TmAbs (tstar a)
-  | TmApp (TmAbs a) b => subst_Tm (tstar b …)(tstar a)
-  | TmApp a b => TmApp (tstar a) (tstar b)
-  (* | TmForall a => TmForall (tstar a) *)
-  end.
-
-Lemma par_cong a0 a1 b0 b1 (h : a0 ⇒ a1) (h1 : b0 ⇒ b1) :
-  subst_Tm (b0…) a0 ⇒ subst_Tm (b1…) a1.
-Proof. auto using par_morphing, par_ρ_ext, par_ρ_id. Qed.
-
-Local Ltac solve_triangle := qauto use:par_refl, par_cong ctrs:Par inv:Par.
-
-Lemma par_triangle a b : a ⇒ b -> b ⇒ tstar a.
-Proof.
-  move : b. apply tstar_ind;
-    hauto lq:on use:par_refl, par_cong ctrs:Par inv:Par.
-Qed.
-
-Lemma par_diamond a b c : a ⇒ b -> a ⇒ c -> b ⇒ tstar a /\ c ⇒ tstar a.
-Proof. auto using par_triangle. Qed.
-
-Lemma pars_diamond : confluent Par.
-Proof.
-  hauto lq:on use:par_diamond, @diamond_confluent unfold:confluent, diamond.
-Qed.
-
-Lemma pars_renaming a b ξ :
-  a ⇒* b ->
-  ren_Tm ξ a ⇒* ren_Tm ξ b.
-Proof.
-  induction 1; hauto lq:on ctrs:rtc use:par_renaming.
-Qed.
-
-Lemma par_subst a b ρ :
-  a ⇒ b ->
-  subst_Tm ρ a ⇒ subst_Tm ρ b.
-Proof.
-  auto using par_refl, par_morphing.
-Qed.
-
-Lemma pars_subst a b ρ :
-  a ⇒* b ->
-  subst_Tm ρ a ⇒* subst_Tm ρ b.
-Proof.
-  induction 1; hauto lq:on ctrs:rtc use:par_subst.
-Qed.
-
-Definition Coherent a b := exists c, a ⇒* c /\ b ⇒* c.
-Infix "⇔" := Coherent (at level 70, no associativity).
-
-
-Lemma coherent_renaming a b ξ :
-  a ⇔ b ->
-  ren_Tm ξ a ⇔ ren_Tm ξ b.
-Proof. hauto lq:on use:pars_renaming unfold:Coherent. Qed.
-
-Lemma coherent_subst a b ρ :
-  a ⇔ b ->
-  subst_Tm ρ a ⇔ subst_Tm ρ b.
-Proof. hauto lq:on use:pars_subst unfold:Coherent. Qed.
-
-Lemma coherent_refl : forall a, a ⇔ a.
-Proof. hauto lq:on use:rtc_refl unfold:Coherent. Qed.
-
-Lemma coherent_sym : forall a b, a ⇔ b -> b ⇔ a.
-Proof. rewrite /Coherent. firstorder. Qed.
-
-Lemma coherent_trans : forall a b c, a ⇔ b -> b ⇔ c -> a ⇔ c.
-Proof.
-  rewrite /Coherent.
-  have h := pars_diamond. rewrite /confluent /diamond in h.
-  move => a b c [ab [ha0 hb0]] [bc [ha1 hb1]].
-  have [abc [hab hbc]] : exists abc, ab ⇒* abc /\ bc ⇒* abc by firstorder.
-  exists abc. eauto using rtc_transitive.
-Qed.
-
-Lemma C_App : ltac2:(gen_cong P_App Coherent).
-Proof. hauto lq:on use:PS_App unfold:Coherent. Qed.
 
 (* Based on https://poplmark-reloaded.github.io/coq/well-scoped/PR.sn_defs.html *)
 Inductive SN : Tm -> Prop :=
